theories/Template/QuoteGround/Coq/Misc.v
@@ -12,9 +12,9 @@ Proof.
   split; destruct v; intuition congruence.
 Defined.
 #[export] Instance quote_forall_eq_some {A v P} {q : ground_quotable (match v return Type with Some v => P v | None => True end)} {qv : quotation_of v} {qA : quotation_of A} {qP : quotation_of P} : ground_quotable (forall a : A, v = Some a -> P a)
-  := quote_of_iffT iff_forall_eq_some.
+  := ground_quotable_of_iffT iff_forall_eq_some.
 #[export] Instance quote_forall_neq_nil {A v P} {q : ground_quotable (match v return Type with nil => True | _ => P end)} {qv : quotation_of v} {qA : quotation_of A} {qP : quotation_of P} : ground_quotable (v <> @nil A -> P)
-  := quote_of_iffT iff_forall_neq_nil.
+  := ground_quotable_of_iffT iff_forall_neq_nil.
 #[export] Instance quote_is_true_or_l {b} {P : Prop} {qP : quotation_of P} {quoteP : ground_quotable P} : ground_quotable (is_true b \/ P).
 Proof.
   apply quote_or_dec_l; try exact _; cbv [is_true]; decide equality.
